

6680210 Problem set 3

collaborators : None

sources consulted : Week 3 Lecture Notes (Canvas)

problem 1

$$(i, j) = (2i) + j$$

i rows, j columns

$$a) \begin{matrix} & j \\ i & \begin{pmatrix} 1 & 2 & 3 \\ 3 & 4 & 5 \\ 5 & 6 & 7 \\ 7 & 8 & 9 \end{pmatrix} \end{matrix}$$

$$b) A^T \Rightarrow \begin{pmatrix} 3 & 5 & 7 \\ 4 & 6 & 8 \\ 5 & 7 & 9 \end{pmatrix}$$

$$c) \text{tr}(A) = 3 + 6 + 9 = 18$$

$$\text{tr}(A^T) = 3 + 6 + 9 = 18$$

yes, they are equal.

$$d) \begin{pmatrix} 3 & 5 & 7 \\ 4 & 6 & 8 \\ 5 & 7 & 9 \end{pmatrix} \xrightarrow{R_1 \leftrightarrow R_2} \begin{pmatrix} 4 & 6 & 8 \\ 3 & 5 & 7 \\ 5 & 7 & 9 \end{pmatrix} \xrightarrow{R_1 = R_1 - R_2} \begin{pmatrix} 1 & 1 & 1 \\ 3 & 5 & 7 \\ 5 & 7 & 9 \end{pmatrix} \xrightarrow{R_2 = R_2 - 3R_1} \begin{pmatrix} 1 & 1 & 1 \\ 0 & 2 & 5 \\ 5 & 7 & 9 \end{pmatrix}$$

$$R_3 = R_3 - 5R_1$$
$$\begin{pmatrix} 1 & 1 & 1 \\ 0 & 2 & 5 \\ 0 & 2 & 4 \end{pmatrix}$$

$$R_2 = R_2 - 0.5R_3$$
$$\begin{pmatrix} 1 & 1 & 1 \\ 0 & 1 & 3 \\ 0 & 2 & 4 \end{pmatrix}$$

$$R_3 = R_3 - R_2$$
$$\begin{pmatrix} 1 & 1 & 1 \\ 0 & 1 & 3 \\ 0 & 1 & 1 \end{pmatrix}$$

$$R_1 = R_1 - R_3$$
$$\begin{pmatrix} 1 & 0 & 0 \\ 0 & 1 & 3 \\ 0 & 1 & 1 \end{pmatrix}$$

$$R_2 = R_2 - R_3$$
$$\begin{pmatrix} 1 & 0 & 0 \\ 0 & 0 & 2 \\ 0 & 1 & 1 \end{pmatrix}$$

$$R_2 \leftrightarrow R_3$$
$$\begin{pmatrix} 1 & 0 & 0 \\ 0 & 1 & 1 \\ 0 & 0 & 2 \end{pmatrix}$$

$$R_3 = \frac{1}{2}R_3$$
$$\begin{pmatrix} 1 & 0 & 0 \\ 0 & 1 & 1 \\ 0 & 0 & 1 \end{pmatrix}$$

$$R_2 = R_2 - R_3$$
$$\begin{pmatrix} 1 & 0 & 0 \\ 0 & 1 & 0 \\ 0 & 0 & 1 \end{pmatrix}$$

✓

## Problem 2

$$B \in \mathbb{R}^{3 \times 4}$$

a)

$$i, j = i^2 \cdot j$$

		j			
i		1	2	3	4
1		1	2	3	4
2		4	8	12	16
3		9	18	27	36

b)

$$B^T = \begin{pmatrix} 1 & 4 & 9 \\ 2 & 8 & 18 \\ 3 & 12 & 27 \\ 4 & 16 & 36 \end{pmatrix}$$

c)

$$\begin{pmatrix} 1 & 2 & 3 & 4 \\ 4 & 8 & 12 & 16 \\ 9 & 18 & 27 & 36 \end{pmatrix} \xrightarrow{R_2 = R_2 - 4R_1} \begin{pmatrix} 1 & 2 & 3 & 4 \\ 0 & 0 & 0 & 0 \\ 9 & 18 & 27 & 36 \end{pmatrix} \xrightarrow{R_3 = R_3 - 9R_1} \begin{pmatrix} 1 & 2 & 3 & 4 \\ 0 & 0 & 0 & 0 \\ 0 & 0 & 0 & 0 \end{pmatrix} \checkmark$$

d)

$$\begin{pmatrix} 1 & 4 & 9 \\ 2 & 8 & 18 \\ 3 & 12 & 27 \\ 4 & 16 & 36 \end{pmatrix} \xrightarrow{R_4 = R_4 - 2R_2} \begin{pmatrix} 1 & 4 & 9 \\ 2 & 8 & 18 \\ 3 & 12 & 27 \\ 0 & 0 & 0 \end{pmatrix} \xrightarrow{R_3 = R_3 - 3R_1} \begin{pmatrix} 1 & 4 & 9 \\ 2 & 8 & 18 \\ 0 & 0 & 0 \\ 0 & 0 & 0 \end{pmatrix} \xrightarrow{R_2 = R_2 - 2R_1} \begin{pmatrix} 1 & 4 & 9 \\ 0 & 0 & 0 \\ 0 & 0 & 0 \\ 0 & 0 & 0 \end{pmatrix} \checkmark$$

### problem 3

$$A = [3] \quad B = [-2] \quad C = [9]$$

a)  $A + B$

$$= 3 + (-2)$$

$$= 1$$

b)  $B - 2 \circ C$

$$= -2 - (2 \circ 9)$$

$$= -20$$

c)  $-3 \circ A + B + 4 \circ C$

$$= (-3 \circ 3) - 2 + (4 \circ 9)$$

$$= -9 - 2 + 36$$

$$= -11 + 36$$

$$= 25$$

d)  $A \circ B$

$$= 3 \circ -2$$

$$= -6$$

e)  $B \circ C$

$$= -2 \circ 9$$

$$= -18$$

f)  $\text{tr}(A+B) + \text{tr}(C^T)$

$$\text{tr}(1) = 1 \Rightarrow \text{tr}(C^T) = \text{tr}(9) = 9$$

$$= 1 + 9$$

$$= 10$$

g)  $(A+B) \circ (B+C)$

$$= 1 \circ 7$$

$$= 7$$

h)  $2AB - 3AC + 4BC$

$$= (2)(3)(-2) - (3)(2)(9) + 4(-2)(9)$$

$$= -12 - 54 - 72$$

$$= -138$$

### Problem 4

$$A = [0 \ 1 \ -1 \ -2] \quad B = [2 \ -1 \ 3 \ -5] \quad C = [3 \ 0 \ -2 \ 3]$$

a)  $-A + B - 2C$

$$\begin{aligned} & -[0 \ 1 \ -1 \ -2] + [2 \ -1 \ 3 \ -5] - 2[3 \ 0 \ -2 \ 3] \\ &= [0 \ -1 \ 1 \ 2] + [2 \ -1 \ 3 \ -5] - [6 \ 0 \ -4 \ 6] \\ &= [-4 \ -2 \ 8 \ -9] \end{aligned}$$

b)  $-3A^T + 4C^T$

$$\begin{aligned} A^T &= \begin{pmatrix} 0 \\ 1 \\ -1 \\ -2 \end{pmatrix} & C^T &= \begin{pmatrix} 3 \\ 0 \\ -2 \\ 3 \end{pmatrix} \\ -3A^T &= \begin{pmatrix} 0 \\ -3 \\ 3 \\ 6 \end{pmatrix} & 4C^T &= \begin{pmatrix} 12 \\ 0 \\ -8 \\ 12 \end{pmatrix} & -3A^T + 4C^T &= \begin{pmatrix} 12 \\ -3 \\ -5 \\ 18 \end{pmatrix} \end{aligned}$$

c)  $1 \times 4$  matrices with 1 row and 4 columns each

d)  $4 \times 1$  matrices with 4 rows and 1 column each

e)  $A \circ B^T$

$$\begin{aligned} A &= [0 \ 1 \ -1 \ -2] & B^T &= \begin{pmatrix} 2 \\ -1 \\ 3 \\ -5 \end{pmatrix} & A \circ B^T &= (0 \cdot 2 + 1 \cdot -1 + -1 \cdot 3 + -2 \cdot -5) \\ & & & & &= 0 - 1 - 3 + 10 \\ & & & & &= -4 + 10 \\ & & & & &= 6 \\ & & & & &\Downarrow \\ & & & & &(6) \end{aligned}$$

$$f) B \circ A^T$$

$$B = (2 \ -1 \ 3 \ -5) \quad A^T = \begin{pmatrix} 0 \\ 1 \\ -1 \\ -2 \end{pmatrix} \quad B \circ A^T = (2 \cdot 0 + -1 \cdot 1 + 3 \cdot -1 + -5 \cdot -2) \\ = 0 - 1 - 3 + 10 \\ = 6 \\ = (6)$$

$$g) B^T \circ C$$

$$B^T = \begin{pmatrix} 2 \\ -1 \\ 3 \\ -5 \end{pmatrix} \quad C = (3 \ 0 \ -2 \ 3) \quad B^T \circ C = \begin{pmatrix} 6 & 0 & -4 & 6 \\ -3 & 0 & 2 & -3 \\ 9 & 0 & -6 & 9 \\ -15 & 0 & 10 & -15 \end{pmatrix}$$

$$h) C^T \circ B$$

$$C^T = \begin{pmatrix} 3 \\ 0 \\ -2 \\ 3 \end{pmatrix} \quad B = (2 \ -1 \ 3 \ -5) \quad C^T \circ B = \begin{pmatrix} 6 & -3 & 9 & -15 \\ 0 & 0 & 0 & 0 \\ -4 & 2 & -6 & 10 \\ 6 & -3 & 9 & -15 \end{pmatrix}$$

$$i) (A+B) \circ (B+C)^T$$

$$A+B = [2 \ 0 \ 2 \ -7] \quad B+C = [5 \ -1 \ 1 \ -2]$$

$$(B+C)^T = \begin{pmatrix} 5 \\ -1 \\ 1 \\ 2 \end{pmatrix}$$

$$(A+B) \circ (B+C)^T$$

$$= (2 \cdot 5 + 0 \cdot -1 + 2 \cdot 1 + -7 \cdot 2)$$

$$= 10 - 1 + 2 - 14$$

$$= -4 - 1 + 2$$

$$= (-3)$$

$$j) (A+B)^T \circ (B+C)$$

$$(A+B)^T = \begin{pmatrix} 2 \\ 0 \\ 2 \\ -7 \end{pmatrix} \quad (B+C) = [5 \ -1 \ 1 \ -2]$$

$$(A+B)^T \circ (B+C) = \begin{pmatrix} 10 & -2 & 2 & -4 \\ 0 & 0 & 0 & 0 \\ 10 & -2 & 2 & -4 \\ -35 & 7 & -7 & 14 \end{pmatrix}$$

### Problem 5

$$X = \begin{bmatrix} 2 & -5 & 0 & 1 \\ 0 & 7 & -3 & -2 \end{bmatrix} \quad Y = \begin{bmatrix} -1 & 8 & 0 & 4 \\ -2 & -6 & 3 & 2 \end{bmatrix}$$

a)  $X + Y$

$$= \begin{bmatrix} 1 & 3 & 0 & 5 \\ -2 & 1 & 0 & 0 \end{bmatrix}$$

b)  $-X^T + 2 \cdot Y^T$

$$X^T = \begin{pmatrix} 2 & 0 \\ -5 & 7 \\ 0 & -3 \\ 1 & -2 \end{pmatrix} \quad -X^T = \begin{pmatrix} -2 & 0 \\ 5 & -7 \\ 0 & 3 \\ -1 & 2 \end{pmatrix} \quad Y^T = \begin{pmatrix} -1 & -2 \\ 8 & -6 \\ 0 & 3 \\ 4 & 2 \end{pmatrix} \quad 2Y^T = \begin{pmatrix} -2 & -4 \\ 16 & -12 \\ 0 & 6 \\ 8 & 4 \end{pmatrix}$$

$$\downarrow$$

$$-X^T + 2Y^T$$

$$\begin{pmatrix} -4 & -4 \\ 21 & -19 \\ 0 & 9 \\ 7 & 6 \end{pmatrix}$$

## Problem 6

$$M = \begin{bmatrix} 0 & 2 & -3 \\ -1 & 0 & 2 \\ 2 & 0 & 1 \end{bmatrix} \quad N = \begin{bmatrix} -3 & 0 & 1 \\ 0 & 2 & 2 \\ -1 & 0 & 0 \end{bmatrix}$$

a)  $M \circ N$

$$= \begin{bmatrix} -3 & 4 & 4 \\ 1 & 0 & -1 \\ -7 & 0 & 2 \end{bmatrix}$$

$$(1,1) = 0 \cdot -3 + 2 \cdot 0 + -3 \cdot 1 = -3$$

$$(1,2) = 0 \cdot 0 + 2 \cdot 2 + -3 \cdot 0 = 4$$

$$(1,3) = 0 \cdot 1 + 2 \cdot 2 + -3 \cdot 0 = 4$$

$$(2,1) = -1 \cdot -3 + 0 \cdot 0 + 2 \cdot 1 = 3 + 2 = 5$$

$$(2,2) = -1 \cdot 0 + 0 \cdot 2 + 2 \cdot 0 = 0$$

$$(2,3) = -1 \cdot 1 + 0 \cdot 2 + 2 \cdot 0 = -1$$

$$(3,1) = 2 \cdot -3 + 0 \cdot 0 + 1 \cdot 1 = -6 + 1 = -5$$

$$(3,2) = 2 \cdot 0 + 0 \cdot 2 + 1 \cdot 0 = 0$$

$$(3,3) = 2 \cdot 1 + 0 \cdot 2 + 1 \cdot 0 = 2$$

b)  $N \circ M$

$$N = \begin{bmatrix} -3 & 0 & 1 \\ 0 & 2 & 2 \\ -1 & 0 & 0 \end{bmatrix} \quad M = \begin{bmatrix} 0 & 2 & -3 \\ -1 & 0 & 2 \\ 2 & 0 & 1 \end{bmatrix}$$

$$N \cdot M$$

$$\begin{bmatrix} 2 & -6 & 10 \\ 2 & 0 & 6 \\ 0 & -2 & 3 \end{bmatrix}$$

$$(1,1) = -3 \cdot 0 + 0 \cdot -1 + 1 \cdot 2 = 2$$

$$(1,2) = -3 \cdot 2 + 0 \cdot 0 + 1 \cdot 0 = -6$$

$$(1,3) = -3 \cdot -3 + 0 \cdot 2 + 1 \cdot 1 = 10$$

$$(2,1) = 0 \cdot 0 + 2 \cdot -1 + 2 \cdot 2 = -2 + 4 = 2$$

$$(2,2) = 0 \cdot 2 + 2 \cdot 0 + 2 \cdot 0 = 0$$

$$(2,3) = 0 \cdot -3 + 2 \cdot 2 + 2 \cdot 1 = 4 + 2 = 6$$

$$(3,1) = -1 \cdot 0 + 0 \cdot -1 + 0 \cdot 2 = 0$$

$$(3,2) = -1 \cdot 2 + 0 \cdot 0 + 0 \cdot 0 = -2$$

$$(3,3) = -1 \cdot -3 + 0 \cdot 2 + 0 \cdot 1 = 3$$

c) Don't feel like doing extra credit ;)



# Problem 7

$$A = \begin{bmatrix} 5 & 2 & 1 \\ 0 & 4 & 3 \end{bmatrix}$$

a)  $A \cdot A^T$

$$A^T = \begin{bmatrix} 5 & 0 \\ 2 & 4 \\ 1 & 3 \end{bmatrix}$$

$$A = \begin{bmatrix} 5 & 2 & 1 \\ 0 & 4 & 3 \end{bmatrix}$$

$$A \cdot A^T = \begin{pmatrix} 30 & 11 \\ 11 & 25 \end{pmatrix}$$

$$(1,1) = 5 \cdot 5 + 2 \cdot 2 + 1 \cdot 1 = 30$$

$$(1,2) = 5 \cdot 0 + 4 \cdot 2 + 3 \cdot 1 = 11$$

$$(2,1) = 0 \cdot 5 + 4 \cdot 2 + 3 \cdot 1 = 11$$

$$(2,2) = 0 \cdot 0 + 4 \cdot 4 + 3 \cdot 3 = 25$$

b)  $A^T \cdot A$

$$A^T = \begin{bmatrix} 5 & 0 \\ 2 & 4 \\ 1 & 3 \end{bmatrix}$$

$$A = \begin{bmatrix} 5 & 2 & 1 \\ 0 & 4 & 3 \end{bmatrix}$$

$$A^T \cdot A = \begin{pmatrix} 25 & 10 & 5 \\ 10 & 20 & 14 \\ 5 & 14 & 10 \end{pmatrix}$$

$$(1,1) = 5 \cdot 5 + 0 \cdot 0 = 25$$

$$(1,2) = 5 \cdot 2 + 0 \cdot 4 = 10$$

$$(1,3) = 5 \cdot 1 + 0 \cdot 3 = 5$$

$$(2,1) = 2 \cdot 5 + 4 \cdot 0 = 10$$

$$(2,2) = 2 \cdot 2 + 4 \cdot 4 = 20$$

$$(2,3) = 2 \cdot 1 + 4 \cdot 3 = 14$$

$$(3,1) = 1 \cdot 5 + 3 \cdot 0 = 5$$

$$(3,2) = 1 \cdot 2 + 3 \cdot 4 = 14$$

$$(3,3) = 1 \cdot 1 + 3 \cdot 3 = 10$$

c)  $\text{tr}(A \cdot A^T) = 30 + 25 = 55$

$$\text{tr}(A^T \cdot A) = 25 + 20 + 10 = 55$$

Yes, they are the same.